Deploying to gh-pages from @ xubaiw/reservoir-index@e3f68601a9abc50450389f9ff12699fd9ca6ff4a 🚀

git/cruhland/lean4-axiomatic/Lean4Axiomatic/AbstractAlgebra.lean
@@ -1,20 +1,9 @@
+import Lean4Axiomatic.AbstractAlgebra.Substitutive
 import Lean4Axiomatic.Eqv
 
-open Relation (EqvOp Refl Swap Symm Trans)
+open Relation (EqvOp)
 
 namespace AA
-
-inductive Hand where
-| L | R
-
-def forHand {α : Sort u} {β : Sort v} : Hand → (α → α → β) → (α → α → β)
-| Hand.L => id
-| Hand.R => flip
-
-class Commutative {α : Sort u} {β : Sort v} [EqvOp β] (f : α → α → β) where
-  comm {x y : α} : f x y ≃ f y x
-
-export Commutative (comm)
 
 /--
 Class for types and operations that satisfy the associative property.
@@ -46,129 +35,6 @@ class Associative {α : Sort u} [EqvOp α] (f : α → α → α) where
   assoc {x y z : α} : f (f x y) z ≃ f x (f y z)
 
 export Associative (assoc)
-
-class Substitutive
-    {α : Sort u} {β : Sort v}
-    (f : α → β) (rα : outParam (α → α → Prop)) (rβ : β → β → Prop) where
-  subst {x₁ x₂ : α} : rα x₁ x₂ → rβ (f x₁) (f x₂)
-
-export Substitutive (subst)
-
-class Injective
-    {α : Sort u} {β : Sort v} (f : α → β)
-    (rα : outParam (α → α → Prop)) (rβ : β → β → Prop) where
-  inject {x₁ x₂ : α} : rβ (f x₁) (f x₂) → rα x₁ x₂
-
-export Injective (inject)
-
-class SubstitutiveForHand
-    (hand : Hand) {α : Sort u} {β : Sort v} (f : α → α → β)
-    (rα : outParam (α → α → Prop)) (rβ : β → β → Prop) where
-  subst₂
-    {x₁ x₂ y : α} : rα x₁ x₂ → rβ (forHand hand f x₁ y) (forHand hand f x₂ y)
-
-export SubstitutiveForHand (subst₂)
-
-abbrev substL := @subst₂ Hand.L
-abbrev substR := @subst₂ Hand.R
-
-class Substitutive₂
-    {α : Sort u} {β : Sort v}
-    (f : α → α → β) (rα : α → α → Prop) (rβ : β → β → Prop)
-    where
-  substitutiveL : SubstitutiveForHand Hand.L f rα rβ
-  substitutiveR : SubstitutiveForHand Hand.R f rα rβ
-
-attribute [instance] Substitutive₂.substitutiveL
-attribute [instance] Substitutive₂.substitutiveR
-
-instance
-    {α : Type u} {β : Type v} {f : α → α → β} {rel : β → β → Prop}
-    [EqvOp β] [Commutative f] [Relation.Refl rel]
-    [SubstitutiveForHand Hand.R rel (· ≃ ·) (· → ·)]
-    : Swap f rel where
-  swap := by
-    intro x y
-    show rel (f x y) (f y x)
-    have : rel (f x y) (f x y) := Eqv.refl
-    exact substR (rβ := (· → ·)) comm ‹rel (f x y) (f x y)›
-
-def substR_from_substL_swap
-    {α : Sort u} {β : Sort v} {f : α → α → β}
-    {rα : α → α → Prop} {rβ : β → β → Prop}
-    [Trans rβ] [Swap f rβ]
-    : SubstitutiveForHand Hand.L f rα rβ →
-    SubstitutiveForHand Hand.R f rα rβ := by
-  intro
-  constructor
-  intro x₁ x₂ y (_ : rα x₁ x₂)
-  show rβ (f y x₁) (f y x₂)
-  calc
-    rβ (f y x₁) (f x₁ y) := Swap.swap
-    rβ (f x₁ y) (f x₂ y) := AA.substL ‹rα x₁ x₂›
-    rβ (f x₂ y) (f y x₂) := Swap.swap
-
-instance eqv_substL {α : Sort u} [EqvOp α]
-    : SubstitutiveForHand Hand.L (α := α) (· ≃ ·) (· ≃ ·) (· → ·) := by
-  constructor
-  intro x₁ x₂ y (_ : x₁ ≃ x₂) (_ : x₁ ≃ y)
-  show x₂ ≃ y
-  exact Eqv.trans (Eqv.symm ‹x₁ ≃ x₂›) ‹x₁ ≃ y›
-
-instance eqv_substR {α : Sort u} [EqvOp α]
-    : SubstitutiveForHand Hand.R (α := α) (· ≃ ·) (· ≃ ·) (· → ·) :=
-  substR_from_substL_swap eqv_substL
-
-instance eqv_substitutive {α : Sort u} [EqvOp α]
-    : Substitutive₂ (α := α) (· ≃ ·) (· ≃ ·) (· → ·) where
-  substitutiveL := eqv_substL
-  substitutiveR := eqv_substR
-
-instance neq_substL
-    {α : Sort u} [EqvOp α]
-    : SubstitutiveForHand Hand.L (α := α) (· ≄ ·) (· ≃ ·) (· → ·) := by
-  constructor
-  intro x₁ x₂ y (_ : x₁ ≃ x₂) (_ : x₁ ≄ y) (_ : x₂ ≃ y)
-  show False
-  apply ‹x₁ ≄ y›
-  show x₁ ≃ y
-  exact Eqv.trans ‹x₁ ≃ x₂› ‹x₂ ≃ y›
-
-instance neq_substitutive
-    {α : Sort u} [EqvOp α] : Substitutive₂ (α := α) (· ≄ ·) (· ≃ ·) (· → ·)
-    where
-  substitutiveL := neq_substL
-  substitutiveR := substR_from_substL_swap neq_substL
-
-class Cancellative
-    (hand : Hand) {α : Sort u} {β : Sort v}
-    (f : α → α → β) (rα : outParam (α → α → Prop)) (rβ : β → β → Prop) where
-  cancel
-    {x y₁ y₂ : α} : rβ (forHand hand f x y₁) (forHand hand f x y₂) → rα y₁ y₂
-
-export Cancellative (cancel)
-
-abbrev cancelL := @cancel Hand.L
-abbrev cancelR := @cancel Hand.R
-
-class Cancellative₂
-    {α : Sort u} {β : Sort v}
-    (f : α → α → β) (rα : outParam (α → α → Prop)) (rβ : β → β → Prop) where
-  cancellativeL : Cancellative Hand.L f rα rβ
-  cancellativeR : Cancellative Hand.R f rα rβ
-
-def cancelR_from_cancelL
-    {α : Sort u} {β : Sort v}
-    {f : α → α → β} {rα : α → α → Prop} {rβ : β → β → Prop}
-    [EqvOp β] [Commutative f] [Substitutive₂ rβ (· ≃ ·) (· → ·)]
-    : Cancellative Hand.L f rα rβ → Cancellative Hand.R f rα rβ := by
-  intro
-  constructor
-  intro x y₁ y₂ (hyp : rβ (f y₁ x) (f y₂ x))
-  show rα y₁ y₂
-  have : rβ (f x y₁) (f y₂ x) := AA.substL (rβ := (· → ·)) AA.comm hyp
-  have : rβ (f x y₁) (f x y₂) := AA.substR (rβ := (· → ·)) AA.comm this
-  exact AA.cancelL this
 
 /--
 Class for types and operations that satisfy either the left- or right-handed
