git/cruhland/lean4-axiomatic/Lean4Axiomatic/AbstractAlgebra/Commutative.lean
@@ -1,0 +1,12 @@
+import Lean4Axiomatic.Eqv
+
+open Relation (EqvOp)
+
+namespace AA
+
+class Commutative {α : Sort u} {β : Sort v} [EqvOp β] (f : α → α → β) where
+  comm {x y : α} : f x y ≃ f y x
+
+export Commutative (comm)
+
+end AA
