git/cruhland/lean4-axiomatic/Lean4Axiomatic/AbstractAlgebra/Core.lean
@@ -1,0 +1,37 @@
+namespace AA
+
+/-!
+# Core definitions
+
+These are used frequently by other abstract algebra definitions.
+-/
+
+/--
+Handedness: either left-handed or right-handed.
+
+This is used by algebra concepts that can be defined for a particular side of a
+binary operator. For example, the concept of a left inverse (`a⁻¹ * a ≃ 1`) vs.
+a right inverse (`a * a⁻¹ ≃ 1`).
+-/
+inductive Hand where
+| /-- Left hand.  -/ L
+| /-- Right hand. -/ R
+
+/--
+Defines a convention for which side of a binary operator its first argument is
+sent to.
+
+The given operator, of type `α → α → β`, is assumed to be left-handed; i.e.,
+its first argument is on the left when written infix. This function outputs a
+modified operator that puts the first argument on whatever side is specified by
+the `Hand` argument.
+
+This allows both the left- and right-handed versions of an algebraic property
+to share a single definition, avoiding repetitive code. See `AA.DistributiveOn`
+for an example.
+-/
+def forHand {α : Sort u} {β : Sort v} : Hand → (α → α → β) → (α → α → β)
+| Hand.L => id
+| Hand.R => flip
+
+end AA
