git/cruhland/lean4-axiomatic/Lean4Axiomatic/Natural.lean
@@ -28,6 +28,10 @@ export Multiplication (
   mul_associative mul_commutative mul_distributive mulOp mul_positive
   mul_substitutive mul_zero step_mul zero_mul zero_product_split
 )
+export Order (
+  le_antisymm le_defn le_reflexive le_split le_transitive leOp
+  lt_defn lt_defn_add ltOp lt_split lt_step lt_step_le lt_zero trichotomy
+)
 export Sign (Positive positive_add positive_defn positive_step)
 
 end Lean4Axiomatic.Natural
