git/xubaiw/BaseN.lean/test.lean
@@ -1,0 +1,23 @@
+import BaseN
+
+open BaseN
+
+def tests : List (String × String) := [
+  ("", ""),
+  ("f", "Zg=="),
+  ("fo", "Zm8="),
+  ("foo", "Zm9v"),
+  ("foob", "Zm9vYg=="),
+  ("fooba", "Zm9vYmE="),
+  ("foobar",  "Zm9vYmFy")
+]
+
+def main : IO Unit := do
+  for t in tests do
+    if encode64 t.fst.toUTF8 ≠ t.snd then
+      throw $ IO.userError s!"Failed encoding: {t.fst} → {t.snd}"
+    if let some x := decode64 t.snd then
+      if String.fromUTF8Unchecked x ≠ t.fst then
+        throw $ IO.userError s!"Failed decoding: {t.snd} → {t.fst}"
+    else 
+      throw $ IO.userError s!"Failed decoding: {t.snd} → {t.fst}"
