git/xubaiw/BaseN.lean/README.md
@@ -1,0 +1,39 @@
+# BaseN.lean
+
+Encoding and decoding for `base16`, `base32`, `base32hex`, `base64` and `base64url`, compliant to [RFC 4648](https://datatracker.ietf.org/doc/html/rfc4648). 
+
+## Usage
+
+```lean
+import BaseN
+open BaseN
+
+#eval encode64 "Man".toUTF8  -- "TWFu"
+#eval decode64 "TWFu" |>.map String.fromUTF8Unchecked  -- some "Man"
+
+#eval encode64 "Ma".toUTF8  -- "TWE="
+#eval decode64 "TWE=" |>.map String.fromUTF8Unchecked  -- some "Ma"
+```
+
+To customize alphabet and other configutation:
+
+```lean
+
+let myAlphabet := {
+  list := "ABCDEFGHIJKLMNOPQRSTUV0123456789".data  -- length of `list` can be 16, 32 or 64
+  padChar := '='  -- padChar can be `none` when list.length = 16
+}  -- all character in `list` and `padChar` should be distinct to each other
+
+def myEncode32 := encodeConfig {
+  alphabet := myAlphabet
+  usePaddding := false  -- do not pad `=` at the end
+}
+
+def myDecode32 := decodeConfig {
+  alphabet := myAlphabet
+  rejectOutside := false  -- ignore characters not in alphabet, otherwise fail the decoding
+}
+
+#eval myEncode32 "Ma".toUTF8
+#eval myDecode32 "E70B" |>.map String.fromUTF8Unchecked
+```
